src/cbor/pulse/raw/everparse/CBOR.Pulse.Raw.EverParse.Det.Impl.fsti
@@ -8,6 +8,7 @@ module Spec = CBOR.Spec.API.Format
 module AP = Pulse.Lib.ArrayPtr
 module SZ = FStar.SizeT
 module U8 = FStar.UInt8
+module U64 = FStar.UInt64
 module Trade = Pulse.Lib.Trade.Util
 
 val cbor_det_match: perm -> cbor_det_t -> Spec.cbor -> slprop
@@ -32,3 +33,22 @@ val cbor_det_get_tagged_payload (_: unit) : get_tagged_payload_t cbor_det_match
 
 val cbor_det_mk_simple_value (_: unit) : mk_simple_t cbor_det_match
 val cbor_det_mk_int64 (_: unit) : mk_int64_t cbor_det_match
+
+(* Field readers *)
+val cbor_det_read_simple_value (_: unit) : read_simple_value_t cbor_det_match
+val cbor_det_read_uint64 (_: unit) : read_uint64_t cbor_det_match
+val cbor_det_get_string_length (_: unit) : get_string_length_t cbor_det_match
+val cbor_det_get_tagged_tag (_: unit) : get_tagged_tag_t cbor_det_match
+val cbor_det_get_array_length (_: unit) : get_array_length_t cbor_det_match
+val cbor_det_get_map_length (_: unit) : get_map_length_t cbor_det_match
+
+(* Elim functions *)
+val cbor_det_elim_simple (_: unit) : elim_simple_t cbor_det_match
+val cbor_det_elim_int64 (_: unit) : elim_int64_t cbor_det_match
+
+(* Reset perm *)
+val cbor_det_reset_perm (_: unit) : reset_perm_t u#0 u#0 cbor_det_match
+
+(* Constructors *)
+val cbor_det_mk_tagged (_: unit) : mk_tagged_t cbor_det_match
+val cbor_det_mk_string (_: unit) : mk_string_t cbor_det_match
